\documentclass[12pt]{book} 

\usepackage{amsmath}
\usepackage{graphicx}
\usepackage{import}
\usepackage{amsfonts}
\usepackage{booktabs}

\setlength{\parindent}{0em}  % sets auto indent at new paragraph to none

\newcommand{\incfig}[1]{%
        \import{./figures/}{#1.pdf_tex}
}

\newcommand{\incimg}[2]{%
       \begin{figure}[h]
               \centering
               \includegraphics[scale = #2]{./figures/#1}
       \end{figure}
}

\title{\coursetitle\linebreak\lecturename}
\author{\\Cain Susko\\ 
           \\ \\ \\
      Queen's University 
    \\School of Computing\\} 

%=-=-=-=-=-title-=-=-=-=-=%
\newcommand{\lecturename}{lID}
\newcommand{\coursetitle}{cID}
%=-=-=-=-=-#####-=-=-=-=-=%

\begin{document}
\begin{titlepage}
        \maketitle
\end{titlepage}


\section*{Example}
grammars can have if/else statements.

for example:
\[S \to iEtS \mid iEtSeS \mid a\]

where $i$ is if, $t$ is then, and $e$ is else.

we can then apply left factoring on the grammar as, it cannot be parsed with recursive descent parsing, which we want.
It would result in 
\[S \to iEtSS' \mid a\]
\[S' \to eS \mid a\]

but we still cannot use recursive descent parsing on this grammar as: $e \in FOLLOW(S')$
\[S \implies iEtSS'\implies iEtiEtSS'S' \implies iEtiEtSS'eS\]

it violates RD2.

\section*{Left Recursive Productions}
given the grammar:
\[<expr> \to <expr> + <term> \mid <term>\]
\[<term> \to ...\]

in this grammar, the parser goes into an infinite loop when $<expr>$ is at the top of the stack.
we an then modify the rules to avoid this.
\[<expr> \to <term> <expTail>\]
\[<expTail> \to + <tem><expTail> \mid \epsilon\]

However, left recursion can be sometimes be replaced by right recursion.

\section*{Eliminate Left Recursion}
the forula for eliminating left recursion from a grammar is:
\[A \to A\alpha_1 \mid ... \mid A\alpha_m\mid B_1\mid ...\mid B_n\]
where $B_i$ does not begin with $A$, $\alpha_j \neq \epsilon, i \leq j \leq m$
such that:
\[A\to B_iA' \mid ... \mid B_nA'\]
\[A' \to \alpha_1 A' \mid ... \mid \alpha_m A' \mid \epsilon\]

\section*{Example}
given the grammar:
\[S \to bSa \mid ccaSb \mid ccbSa \mid abc \mid \epsilon\]
we can use left factoring and recursion elimination to convert it to the following grammar:
\begin{align*}
        S &\to ccS' \mid abc \mid \epsilon \mid bSa\\
        S' &\to aSb \mid bSa
\end{align*}
\section*{Example}
given:
\[S \to Sabc \mid Sabd \mid ccb \mid cca\]
we will first elimiate the left recursion:
\[S \to ccbS' \mid ccaS'\;\;\;\;S' \to abcS' \mid abdS' \mid \epsilon\]

we will then do left factoring twice (as we can see that there are 2 common prefixes in the new above grammar: $cc, ab$)
\[ \;\;\;\; \]
\begin{align*}
        S &\to ccX\\
        X &\to bS' \mid aS'\\
        S' &\to abY \mid \epsilon \\
        Y &\to cS' \mid dS'
\end{align*}
\end{document}

